theories/Word.ec
@@ -1,12 +1,13 @@
 require        Bool.
-require        Bitstring.
+require import Bitstring.
 require import Int.
 
 cnst k: int.
 axiom k_pos: 0 <= k.
 
-require import Array.
 clone Bitstring as Word.
+export Bitstring.
+
 type word = Word.bitstring.
 
 axiom fixed_length: forall (w:word), Word.length w = k.
